src/coq/Semantics/TopLevel.v
@@ -10,6 +10,7 @@ From ITree Require Import
      Events.State.
 
 From ExtLib Require Import
+     Structures.Functor
      Structures.Monads
      Data.Map.FMapAList.
 
@@ -139,8 +140,8 @@ Module Type LLVMTopLevel (IS : InterpreterStack).
 
   Notation res_L1 := (global_env * dvalue)%type.
   Notation res_L2 := (local_env * lstack * res_L1)%type.
-  Notation res_L3 := (MemState * res_L2)%type.
-  Notation res_L4 := (MemState * (local_env * lstack * (global_env * dvalue)))%type.
+  Notation res_L3 := (MemState * (Provenance * (store_id * res_L2)))%type.
+  Notation res_L4 := (MemState * (Provenance * (store_id * (local_env * lstack * (global_env * dvalue)))))%type.
 
   (**
      Full denotation of a Vellvm program as an interaction tree:
@@ -187,23 +188,21 @@ Module Type LLVMTopLevel (IS : InterpreterStack).
      the resulting [itree].
    *)
   Definition interpreter_gen
-             {MemM : Type -> Type}
-             `{MemMonad MemState AllocationId MemM}
              (ret_typ : dtyp)
              (entry : string)
              (args : list uvalue)
              (prog: list (toplevel_entity typ (block typ * list (block typ))))
     : itree L4 res_L4 :=
     let t := denote_vellvm ret_typ entry args (convert_types (mcfg_of_tle prog)) in
-    interp_mcfg4_exec t [] ([],[]) initial_memory_state.
+    interp_mcfg4_exec t [] ([],[]) 0 initial_provenance initial_memory_state.
 
   (**
      Finally, the reference interpreter assumes no user-defined intrinsics and starts 
      from "main" using bogus initial inputs.
    *)
-  Definition interpreter {MemM : Type -> Type}
-             `{MemMonad MemState AllocationId MemM}
-    := interpreter_gen (DTYPE_I 32%N) "main" main_args.
+  Definition interpreter
+             (prog : list (toplevel_entity typ (block typ * list (block typ)))) : itree L4 res_L4
+    := interpreter_gen (DTYPE_I 32%N) "main" main_args prog.
 
   (**
      We now turn to the definition of our _model_ of vellvm's semantics. The
@@ -221,9 +220,9 @@ Module Type LLVMTopLevel (IS : InterpreterStack).
              (entry : string)
              (args : list uvalue)
              (prog: list (toplevel_entity typ (block typ * list (block typ))))
-    : PropT L4 (MemState * (local_env * lstack * (global_env * dvalue))) :=
+    : PropT L4 res_L4 :=
     let t := denote_vellvm ret_typ entry args (convert_types (mcfg_of_tle prog)) in
-    ℑs eq eq t [] ([],[]) initial_memory_state. 
+    ℑs eq eq t [] ([],[]) 0 initial_provenance initial_memory_state. 
 
   (**
      Finally, the official model assumes no user-defined intrinsics.
